src/lowparse/pulse/LowParse.Pulse.VCList.fst
@@ -185,9 +185,9 @@ ensures exists* v' .
   synth_inverse_2 t (n - 1);
   Trade.rewrite_with_trade
     (pts_to_serialized (serialize_nlist n s) input #pm v)
-    (pts_to_serialized (serialize_synth _ (synth_nlist (n - 1)) (serialize_nondep_then s (serialize_nlist' (n - 1) s)) (synth_nlist_recip (n - 1)) ()) input #pm v);
+    (pts_to_serialized (serialize_synth _ (synth_nlist (n - 1)) (serialize_nondep_then s (serialize_nlist (n - 1) s)) (synth_nlist_recip (n - 1)) ()) input #pm v);
   pts_to_serialized_synth_l2r_trade
-    (serialize_nondep_then s (serialize_nlist' (n - 1) s))
+    (serialize_nondep_then s (serialize_nlist (n - 1) s))
     (synth_nlist (n - 1))
     (synth_nlist_recip (n - 1))
     input;
@@ -252,8 +252,11 @@ ensures
   unfold (split_nondep_then_post s (serialize_nlist (n - 1) s) input pm v' (s1, s2));
   unfold (split_nondep_then_post' s (serialize_nlist (n - 1) s) input pm v' s1 s2);
   Trade.trans _ _ (pts_to_serialized (serialize_nlist n s) input #pm v);
+  rewrite each (fst v') as (List.Tot.hd v);
+  rewrite each (snd v') as (List.Tot.tl v);
   fold (nlist_hd_tl_post' s sq n input pm v s1 s2);
-  fold (nlist_hd_tl_post s sq n input pm v res);
+  rewrite (nlist_hd_tl_post' s sq n input pm v s1 s2)
+    as (nlist_hd_tl_post s sq n input pm v res);
   res
 }
 
@@ -380,6 +383,15 @@ ensures (
     hd tl
   );
   Trade.trans _ _ (pts_to_serialized (serialize_nondep_then (serialize_nlist n s) s') input #pm v);
+  with vhd v' . assert (
+  pts_to_serialized s hd #pm vhd **
+  pts_to_serialized (serialize_nondep_then (serialize_nlist (n - 1) s) s') tl #pm v' **
+  Trade.trade
+    (pts_to_serialized s hd #pm vhd **
+  pts_to_serialized (serialize_nondep_then (serialize_nlist (n - 1) s) s') tl #pm v')
+    (pts_to_serialized (serialize_nondep_then (serialize_nlist n s) s') input #pm v)
+  );
+  rewrite each vhd as (List.Tot.hd (fst v));
   (hd, tl)
 }
 
@@ -508,6 +520,33 @@ ensures (
   tl
 }
 
+ghost fn trade_trans_nounify
+  (a1 a2 a2' a3: slprop)
+requires
+  trade a1 a2 ** trade a2' a3 ** pure (a2 == a2')
+ensures
+  trade a1 a3
+{
+  rewrite each a2' as a2;
+  Trade.trans a1 a2 a3
+}
+
+let nlist_nth_inv
+  (#t: Type0)
+  (n0: Ghost.erased nat)
+  (v0: list t)
+  (i0: SZ.t)
+  (i: SZ.t)
+  (n: nat)
+  (v: list t)
+: Tot prop
+= SZ.v i0 < n0 /\
+  SZ.v i <= SZ.v i0 /\
+  n == n0 - SZ.v i /\
+  List.Tot.length v0 == Ghost.reveal n0 /\
+  List.Tot.length v == n /\
+  List.Tot.index v0 (SZ.v i0) == List.Tot.index v (SZ.v i0 - SZ.v i)
+
 inline_for_extraction
 fn nlist_nth
    (#t: Type0)
@@ -549,20 +588,21 @@ ensures exists* v .
     let res = !pres;
     rewrite each 'res as res;
     let i = !pi;
+    with v . assert (pts_to_serialized (serialize_nlist (n0 - SZ.v i) s) res #pm v);
     let res2 = nlist_tl s j (n0 - SZ.v i) res;
     pi := (SZ.add i 1sz);
     pres := res2;
-    Trade.trans
-      (pts_to_serialized (serialize_nlist (n0 - SZ.v i - 1) s) res2 #pm _)
-      _
-      _
+    with v' . assert (pts_to_serialized (serialize_nlist (n0 - SZ.v i - 1) s) res2 #pm v');
+//    rewrite each (n') as (n0 - SZ.v i - 1);
+    trade_trans_nounify _ _ _ 
+      (pts_to_serialized (serialize_nlist n0 s) input #pm v0);
   };
   with 'res. assert R.pts_to pres 'res;
   let res = !pres;
   rewrite each 'res as res;
   let res2 = nlist_hd s j (n0 - SZ.v i0) res;
-  Trade.trans
-    (pts_to_serialized s res2 #pm _) _ _;
+  trade_trans_nounify
+    _ _ _ (pts_to_serialized (serialize_nlist n0 s) input #pm v0);
   res2
 }
 
@@ -608,14 +648,15 @@ ensures
     true
   } else {
     let pl = nlist_hd_tl s sq j (SZ.v n) a;
-    let s1, s2 = pl;
-    unfold (nlist_hd_tl_post s sq (SZ.v n) a pm v pl);
+    norewrite let s1, s2 = pl;
+    rewrite (nlist_hd_tl_post s sq (SZ.v n) a pm v pl) as (nlist_hd_tl_post' s sq (SZ.v n) a pm v s1 s2);
     unfold (nlist_hd_tl_post' s sq (SZ.v n) a pm v s1 s2);
     let mut phd = s1;
     let mut ptl = s2;
     let n' : SZ.t = SZ.sub n 1sz;
     let mut pi = n';
     let mut pres = true;
+    rewrite each (SZ.v n - 1) as SZ.v n';
     while (
       let i = !pi;
       let res = !pres;
@@ -644,8 +685,8 @@ ensures
       rewrite each 'stl as stl;
       with tl . assert (pts_to_serialized (serialize_nlist (SZ.v gi) s) stl #pm tl);
       let pl = nlist_hd_tl s sq j (SZ.v gi) stl;
-      let s1, s2 = pl;
-      unfold (nlist_hd_tl_post s sq (SZ.v gi) stl pm tl pl);
+      norewrite let s1, s2 = pl;
+      rewrite (nlist_hd_tl_post s sq (SZ.v gi) stl pm tl pl) as (nlist_hd_tl_post' s sq (SZ.v gi) stl pm tl s1 s2);
       unfold (nlist_hd_tl_post' s sq (SZ.v gi) stl pm tl s1 s2);
       with 'phd. assert R.pts_to phd 'phd;
       let shd = !phd;
@@ -659,6 +700,8 @@ ensures
         let i = !pi;
         let i' : SZ.t = SZ.sub i 1sz;
         pi := i';
+        rewrite each (SZ.v i - 1) as SZ.v i';
+        ()
       } else {
         Trade.elim _ (pts_to_serialized (serialize_nlist (SZ.v gi) s) stl #pm tl);
         pres := false;
@@ -1395,6 +1438,7 @@ fn l2r_write_nlist_as_slice0
   let n' = S.len arr.v;
   nlist_match_slice_intro Some (fun _ -> vmatch) (SZ.v n') arr x arr c;
   let res = l2r_write_nlist_as_slice Some (fun _ -> vmatch) s (fun _ -> w) n' arr out offset;
+  rewrite each SZ.v n' as n;
   fold (nlist_match_slice0 vmatch (n) arr x);
   res
 }
